---
layout: post
title: "Matrix transpose and inversion."
date: 2017-01-09
categories: [practice]
tags: [linear algebra]
difficulty: 0
---

### Problem ###

Prove for a nonsingular (e.g. square and invertible) matrix that
$$(A^T)^{-1} = (A^{-1})^T$$.

### Solution ###
<a id='answer-toggle' href="#" onclick="toggleDiv()">show</a>

<div id="answer-block"  style="display:none;">
<!---
We have
\begin{align}
I = (AA^{-1})^T = (A^{-1})^T A^T.
\end{align}

Multiplying both sides by $$(A^T)^{-1}$$ gives

\begin{align}
(A^T)^{-1} = (A^{-1})^T A^T (A^T)^{-1} = (A^{-1})^T I = (A^{-1})^T.
\end{align}

-->
</div>
